typinf.mli
@@ -4,6 +4,8 @@ type bool =
 | True
 | False
 
+val negb : bool -> bool
+
 type nat =
 | O
 | S of nat
@@ -23,13 +25,6 @@ val fst : ('a1, 'a2) prod -> 'a1
 
 val snd : ('a1, 'a2) prod -> 'a2
 
-type comparison =
-| Eq
-| Lt
-| Gt
-
-val compOpp : comparison -> comparison
-
 type 'a list =
 | Nil
 | Cons of 'a * 'a list
@@ -37,6 +32,24 @@ type 'a list =
 val length : 'a1 list -> nat
 
 val app : 'a1 list -> 'a1 list -> 'a1 list
+
+type comparison =
+| Eq
+| Lt
+| Gt
+
+val compOpp : comparison -> comparison
+
+type compareSpecT =
+| CompEqT
+| CompLtT
+| CompGtT
+
+val compareSpec2Type : comparison -> compareSpecT
+
+type 'a compSpecT = compareSpecT
+
+val compSpec2Type : 'a1 -> 'a1 -> comparison -> 'a1 compSpecT
 
 type 'a sig0 =
   'a
@@ -54,22 +67,15 @@ val plus : nat -> nat -> nat
 
 val minus : nat -> nat -> nat
 
-module type TotalOrder' = 
- sig 
-  type t 
- end
-
-val eq_nat_dec : nat -> nat -> sumbool
-
-val le_lt_dec : nat -> nat -> sumbool
-
-module MakeOrderTac : 
- functor (O:TotalOrder') ->
- sig 
-  
- end
-
 val max : nat -> nat -> nat
+
+val nat_iter : nat -> ('a1 -> 'a1) -> 'a1 -> 'a1
+
+type reflect =
+| ReflectT
+| ReflectF
+
+val iff_reflect : bool -> reflect
 
 val nth : nat -> 'a1 list -> 'a1 -> 'a1
 
@@ -87,54 +93,853 @@ val combine : 'a1 list -> 'a2 list -> ('a1, 'a2) prod list
 
 val seq : nat -> nat -> nat list
 
+val eq_nat_dec : nat -> nat -> sumbool
+
+val le_lt_dec : nat -> nat -> sumbool
+
 type positive =
 | XI of positive
 | XO of positive
 | XH
 
-val psucc : positive -> positive
-
-val pplus : positive -> positive -> positive
-
-val pplus_carry : positive -> positive -> positive
-
-val pdouble_minus_one : positive -> positive
-
-type positive_mask =
-| IsNul
-| IsPos of positive
-| IsNeg
-
-val pdouble_plus_one_mask : positive_mask -> positive_mask
-
-val pdouble_mask : positive_mask -> positive_mask
-
-val pdouble_minus_two : positive -> positive_mask
-
-val pminus_mask : positive -> positive -> positive_mask
-
-val pminus_mask_carry : positive -> positive -> positive_mask
-
-val pminus : positive -> positive -> positive
-
-val pcompare : positive -> positive -> comparison -> comparison
-
-val positive_eq_dec : positive -> positive -> sumbool
+type n =
+| N0
+| Npos of positive
 
 type z =
 | Z0
 | Zpos of positive
 | Zneg of positive
 
-val zplus : z -> z -> z
+module type TotalOrder' = 
+ sig 
+  type t 
+ end
 
-val zcompare : z -> z -> comparison
+module MakeOrderTac : 
+ functor (O:TotalOrder') ->
+ sig 
+  
+ end
 
-val z_eq_dec : z -> z -> sumbool
+module MaxLogicalProperties : 
+ functor (O:TotalOrder') ->
+ functor (M:sig 
+  val max : O.t -> O.t -> O.t
+ end) ->
+ sig 
+  module Private_Tac : 
+   sig 
+    
+   end
+ end
 
-val zmax : z -> z -> z
+module Pos : 
+ sig 
+  type t = positive
+  
+  val succ : positive -> positive
+  
+  val add : positive -> positive -> positive
+  
+  val add_carry : positive -> positive -> positive
+  
+  val pred_double : positive -> positive
+  
+  val pred : positive -> positive
+  
+  val pred_N : positive -> n
+  
+  type mask =
+  | IsNul
+  | IsPos of positive
+  | IsNeg
+  
+  val mask_rect : 'a1 -> (positive -> 'a1) -> 'a1 -> mask -> 'a1
+  
+  val mask_rec : 'a1 -> (positive -> 'a1) -> 'a1 -> mask -> 'a1
+  
+  val succ_double_mask : mask -> mask
+  
+  val double_mask : mask -> mask
+  
+  val double_pred_mask : positive -> mask
+  
+  val pred_mask : mask -> mask
+  
+  val sub_mask : positive -> positive -> mask
+  
+  val sub_mask_carry : positive -> positive -> mask
+  
+  val sub : positive -> positive -> positive
+  
+  val mul : positive -> positive -> positive
+  
+  val iter : positive -> ('a1 -> 'a1) -> 'a1 -> 'a1
+  
+  val pow : positive -> positive -> positive
+  
+  val square : positive -> positive
+  
+  val div2 : positive -> positive
+  
+  val div2_up : positive -> positive
+  
+  val size_nat : positive -> nat
+  
+  val size : positive -> positive
+  
+  val compare_cont : positive -> positive -> comparison -> comparison
+  
+  val compare : positive -> positive -> comparison
+  
+  val min : positive -> positive -> positive
+  
+  val max : positive -> positive -> positive
+  
+  val eqb : positive -> positive -> bool
+  
+  val leb : positive -> positive -> bool
+  
+  val ltb : positive -> positive -> bool
+  
+  val sqrtrem_step :
+    (positive -> positive) -> (positive -> positive) -> (positive, mask) prod
+    -> (positive, mask) prod
+  
+  val sqrtrem : positive -> (positive, mask) prod
+  
+  val sqrt : positive -> positive
+  
+  val gcdn : nat -> positive -> positive -> positive
+  
+  val gcd : positive -> positive -> positive
+  
+  val ggcdn :
+    nat -> positive -> positive -> (positive, (positive, positive) prod) prod
+  
+  val ggcd :
+    positive -> positive -> (positive, (positive, positive) prod) prod
+  
+  val coq_Nsucc_double : n -> n
+  
+  val coq_Ndouble : n -> n
+  
+  val coq_lor : positive -> positive -> positive
+  
+  val coq_land : positive -> positive -> n
+  
+  val ldiff : positive -> positive -> n
+  
+  val coq_lxor : positive -> positive -> n
+  
+  val shiftl_nat : positive -> nat -> positive
+  
+  val shiftr_nat : positive -> nat -> positive
+  
+  val shiftl : positive -> n -> positive
+  
+  val shiftr : positive -> n -> positive
+  
+  val testbit_nat : positive -> nat -> bool
+  
+  val testbit : positive -> n -> bool
+  
+  val iter_op : ('a1 -> 'a1 -> 'a1) -> positive -> 'a1 -> 'a1
+  
+  val to_nat : positive -> nat
+  
+  val of_nat : nat -> positive
+  
+  val of_succ_nat : nat -> positive
+ end
 
-type 'x compare =
+module Coq_Pos : 
+ sig 
+  type t = positive
+  
+  val succ : positive -> positive
+  
+  val add : positive -> positive -> positive
+  
+  val add_carry : positive -> positive -> positive
+  
+  val pred_double : positive -> positive
+  
+  val pred : positive -> positive
+  
+  val pred_N : positive -> n
+  
+  type mask = Pos.mask =
+  | IsNul
+  | IsPos of positive
+  | IsNeg
+  
+  val mask_rect : 'a1 -> (positive -> 'a1) -> 'a1 -> mask -> 'a1
+  
+  val mask_rec : 'a1 -> (positive -> 'a1) -> 'a1 -> mask -> 'a1
+  
+  val succ_double_mask : mask -> mask
+  
+  val double_mask : mask -> mask
+  
+  val double_pred_mask : positive -> mask
+  
+  val pred_mask : mask -> mask
+  
+  val sub_mask : positive -> positive -> mask
+  
+  val sub_mask_carry : positive -> positive -> mask
+  
+  val sub : positive -> positive -> positive
+  
+  val mul : positive -> positive -> positive
+  
+  val iter : positive -> ('a1 -> 'a1) -> 'a1 -> 'a1
+  
+  val pow : positive -> positive -> positive
+  
+  val square : positive -> positive
+  
+  val div2 : positive -> positive
+  
+  val div2_up : positive -> positive
+  
+  val size_nat : positive -> nat
+  
+  val size : positive -> positive
+  
+  val compare_cont : positive -> positive -> comparison -> comparison
+  
+  val compare : positive -> positive -> comparison
+  
+  val min : positive -> positive -> positive
+  
+  val max : positive -> positive -> positive
+  
+  val eqb : positive -> positive -> bool
+  
+  val leb : positive -> positive -> bool
+  
+  val ltb : positive -> positive -> bool
+  
+  val sqrtrem_step :
+    (positive -> positive) -> (positive -> positive) -> (positive, mask) prod
+    -> (positive, mask) prod
+  
+  val sqrtrem : positive -> (positive, mask) prod
+  
+  val sqrt : positive -> positive
+  
+  val gcdn : nat -> positive -> positive -> positive
+  
+  val gcd : positive -> positive -> positive
+  
+  val ggcdn :
+    nat -> positive -> positive -> (positive, (positive, positive) prod) prod
+  
+  val ggcd :
+    positive -> positive -> (positive, (positive, positive) prod) prod
+  
+  val coq_Nsucc_double : n -> n
+  
+  val coq_Ndouble : n -> n
+  
+  val coq_lor : positive -> positive -> positive
+  
+  val coq_land : positive -> positive -> n
+  
+  val ldiff : positive -> positive -> n
+  
+  val coq_lxor : positive -> positive -> n
+  
+  val shiftl_nat : positive -> nat -> positive
+  
+  val shiftr_nat : positive -> nat -> positive
+  
+  val shiftl : positive -> n -> positive
+  
+  val shiftr : positive -> n -> positive
+  
+  val testbit_nat : positive -> nat -> bool
+  
+  val testbit : positive -> n -> bool
+  
+  val iter_op : ('a1 -> 'a1 -> 'a1) -> positive -> 'a1 -> 'a1
+  
+  val to_nat : positive -> nat
+  
+  val of_nat : nat -> positive
+  
+  val of_succ_nat : nat -> positive
+  
+  val eq_dec : positive -> positive -> sumbool
+  
+  val peano_rect : 'a1 -> (positive -> 'a1 -> 'a1) -> positive -> 'a1
+  
+  val peano_rec : 'a1 -> (positive -> 'a1 -> 'a1) -> positive -> 'a1
+  
+  type coq_PeanoView =
+  | PeanoOne
+  | PeanoSucc of positive * coq_PeanoView
+  
+  val coq_PeanoView_rect :
+    'a1 -> (positive -> coq_PeanoView -> 'a1 -> 'a1) -> positive ->
+    coq_PeanoView -> 'a1
+  
+  val coq_PeanoView_rec :
+    'a1 -> (positive -> coq_PeanoView -> 'a1 -> 'a1) -> positive ->
+    coq_PeanoView -> 'a1
+  
+  val peanoView_xO : positive -> coq_PeanoView -> coq_PeanoView
+  
+  val peanoView_xI : positive -> coq_PeanoView -> coq_PeanoView
+  
+  val peanoView : positive -> coq_PeanoView
+  
+  val coq_PeanoView_iter :
+    'a1 -> (positive -> 'a1 -> 'a1) -> positive -> coq_PeanoView -> 'a1
+  
+  val eqb_spec : positive -> positive -> reflect
+  
+  val switch_Eq : comparison -> comparison -> comparison
+  
+  val mask2cmp : mask -> comparison
+  
+  val leb_spec0 : positive -> positive -> reflect
+  
+  val ltb_spec0 : positive -> positive -> reflect
+  
+  module Private_Tac : 
+   sig 
+    
+   end
+  
+  module Private_Rev : 
+   sig 
+    module ORev : 
+     sig 
+      type t = positive
+     end
+    
+    module MRev : 
+     sig 
+      val max : positive -> positive -> positive
+     end
+    
+    module MPRev : 
+     sig 
+      module Private_Tac : 
+       sig 
+        
+       end
+     end
+   end
+  
+  module Private_Dec : 
+   sig 
+    val max_case_strong :
+      positive -> positive -> (positive -> positive -> __ -> 'a1 -> 'a1) ->
+      (__ -> 'a1) -> (__ -> 'a1) -> 'a1
+    
+    val max_case :
+      positive -> positive -> (positive -> positive -> __ -> 'a1 -> 'a1) ->
+      'a1 -> 'a1 -> 'a1
+    
+    val max_dec : positive -> positive -> sumbool
+    
+    val min_case_strong :
+      positive -> positive -> (positive -> positive -> __ -> 'a1 -> 'a1) ->
+      (__ -> 'a1) -> (__ -> 'a1) -> 'a1
+    
+    val min_case :
+      positive -> positive -> (positive -> positive -> __ -> 'a1 -> 'a1) ->
+      'a1 -> 'a1 -> 'a1
+    
+    val min_dec : positive -> positive -> sumbool
+   end
+  
+  val max_case_strong :
+    positive -> positive -> (__ -> 'a1) -> (__ -> 'a1) -> 'a1
+  
+  val max_case : positive -> positive -> 'a1 -> 'a1 -> 'a1
+  
+  val max_dec : positive -> positive -> sumbool
+  
+  val min_case_strong :
+    positive -> positive -> (__ -> 'a1) -> (__ -> 'a1) -> 'a1
+  
+  val min_case : positive -> positive -> 'a1 -> 'a1 -> 'a1
+  
+  val min_dec : positive -> positive -> sumbool
+ end
+
+module N : 
+ sig 
+  type t = n
+  
+  val zero : n
+  
+  val one : n
+  
+  val two : n
+  
+  val succ_double : n -> n
+  
+  val double : n -> n
+  
+  val succ : n -> n
+  
+  val pred : n -> n
+  
+  val succ_pos : n -> positive
+  
+  val add : n -> n -> n
+  
+  val sub : n -> n -> n
+  
+  val mul : n -> n -> n
+  
+  val compare : n -> n -> comparison
+  
+  val eqb : n -> n -> bool
+  
+  val leb : n -> n -> bool
+  
+  val ltb : n -> n -> bool
+  
+  val min : n -> n -> n
+  
+  val max : n -> n -> n
+  
+  val div2 : n -> n
+  
+  val even : n -> bool
+  
+  val odd : n -> bool
+  
+  val pow : n -> n -> n
+  
+  val square : n -> n
+  
+  val log2 : n -> n
+  
+  val size : n -> n
+  
+  val size_nat : n -> nat
+  
+  val pos_div_eucl : positive -> n -> (n, n) prod
+  
+  val div_eucl : n -> n -> (n, n) prod
+  
+  val div : n -> n -> n
+  
+  val modulo : n -> n -> n
+  
+  val gcd : n -> n -> n
+  
+  val ggcd : n -> n -> (n, (n, n) prod) prod
+  
+  val sqrtrem : n -> (n, n) prod
+  
+  val sqrt : n -> n
+  
+  val coq_lor : n -> n -> n
+  
+  val coq_land : n -> n -> n
+  
+  val ldiff : n -> n -> n
+  
+  val coq_lxor : n -> n -> n
+  
+  val shiftl_nat : n -> nat -> n
+  
+  val shiftr_nat : n -> nat -> n
+  
+  val shiftl : n -> n -> n
+  
+  val shiftr : n -> n -> n
+  
+  val testbit_nat : n -> nat -> bool
+  
+  val testbit : n -> n -> bool
+  
+  val to_nat : n -> nat
+  
+  val of_nat : nat -> n
+  
+  val iter : n -> ('a1 -> 'a1) -> 'a1 -> 'a1
+  
+  val eq_dec : n -> n -> sumbool
+  
+  val discr : n -> positive sumor
+  
+  val binary_rect : 'a1 -> (n -> 'a1 -> 'a1) -> (n -> 'a1 -> 'a1) -> n -> 'a1
+  
+  val binary_rec : 'a1 -> (n -> 'a1 -> 'a1) -> (n -> 'a1 -> 'a1) -> n -> 'a1
+  
+  val peano_rect : 'a1 -> (n -> 'a1 -> 'a1) -> n -> 'a1
+  
+  val peano_rec : 'a1 -> (n -> 'a1 -> 'a1) -> n -> 'a1
+  
+  val leb_spec0 : n -> n -> reflect
+  
+  val ltb_spec0 : n -> n -> reflect
+  
+  module Private_BootStrap : 
+   sig 
+    
+   end
+  
+  val recursion : 'a1 -> (n -> 'a1 -> 'a1) -> n -> 'a1
+  
+  module Private_OrderTac : 
+   sig 
+    module Elts : 
+     sig 
+      type t = n
+     end
+    
+    module Tac : 
+     sig 
+      
+     end
+   end
+  
+  module Private_NZPow : 
+   sig 
+    
+   end
+  
+  module Private_NZSqrt : 
+   sig 
+    
+   end
+  
+  val sqrt_up : n -> n
+  
+  val log2_up : n -> n
+  
+  module Private_NZDiv : 
+   sig 
+    
+   end
+  
+  val lcm : n -> n -> n
+  
+  val eqb_spec : n -> n -> reflect
+  
+  val b2n : bool -> n
+  
+  val setbit : n -> n -> n
+  
+  val clearbit : n -> n -> n
+  
+  val ones : n -> n
+  
+  val lnot : n -> n -> n
+  
+  module Private_Tac : 
+   sig 
+    
+   end
+  
+  module Private_Rev : 
+   sig 
+    module ORev : 
+     sig 
+      type t = n
+     end
+    
+    module MRev : 
+     sig 
+      val max : n -> n -> n
+     end
+    
+    module MPRev : 
+     sig 
+      module Private_Tac : 
+       sig 
+        
+       end
+     end
+   end
+  
+  module Private_Dec : 
+   sig 
+    val max_case_strong :
+      n -> n -> (n -> n -> __ -> 'a1 -> 'a1) -> (__ -> 'a1) -> (__ -> 'a1) ->
+      'a1
+    
+    val max_case :
+      n -> n -> (n -> n -> __ -> 'a1 -> 'a1) -> 'a1 -> 'a1 -> 'a1
+    
+    val max_dec : n -> n -> sumbool
+    
+    val min_case_strong :
+      n -> n -> (n -> n -> __ -> 'a1 -> 'a1) -> (__ -> 'a1) -> (__ -> 'a1) ->
+      'a1
+    
+    val min_case :
+      n -> n -> (n -> n -> __ -> 'a1 -> 'a1) -> 'a1 -> 'a1 -> 'a1
+    
+    val min_dec : n -> n -> sumbool
+   end
+  
+  val max_case_strong : n -> n -> (__ -> 'a1) -> (__ -> 'a1) -> 'a1
+  
+  val max_case : n -> n -> 'a1 -> 'a1 -> 'a1
+  
+  val max_dec : n -> n -> sumbool
+  
+  val min_case_strong : n -> n -> (__ -> 'a1) -> (__ -> 'a1) -> 'a1
+  
+  val min_case : n -> n -> 'a1 -> 'a1 -> 'a1
+  
+  val min_dec : n -> n -> sumbool
+ end
+
+module Z : 
+ sig 
+  type t = z
+  
+  val zero : z
+  
+  val one : z
+  
+  val two : z
+  
+  val double : z -> z
+  
+  val succ_double : z -> z
+  
+  val pred_double : z -> z
+  
+  val pos_sub : positive -> positive -> z
+  
+  val add : z -> z -> z
+  
+  val opp : z -> z
+  
+  val succ : z -> z
+  
+  val pred : z -> z
+  
+  val sub : z -> z -> z
+  
+  val mul : z -> z -> z
+  
+  val pow_pos : z -> positive -> z
+  
+  val pow : z -> z -> z
+  
+  val square : z -> z
+  
+  val compare : z -> z -> comparison
+  
+  val sgn : z -> z
+  
+  val leb : z -> z -> bool
+  
+  val ltb : z -> z -> bool
+  
+  val geb : z -> z -> bool
+  
+  val gtb : z -> z -> bool
+  
+  val eqb : z -> z -> bool
+  
+  val max : z -> z -> z
+  
+  val min : z -> z -> z
+  
+  val abs : z -> z
+  
+  val abs_nat : z -> nat
+  
+  val abs_N : z -> n
+  
+  val to_nat : z -> nat
+  
+  val to_N : z -> n
+  
+  val of_nat : nat -> z
+  
+  val of_N : n -> z
+  
+  val to_pos : z -> positive
+  
+  val iter : z -> ('a1 -> 'a1) -> 'a1 -> 'a1
+  
+  val pos_div_eucl : positive -> z -> (z, z) prod
+  
+  val div_eucl : z -> z -> (z, z) prod
+  
+  val div : z -> z -> z
+  
+  val modulo : z -> z -> z
+  
+  val quotrem : z -> z -> (z, z) prod
+  
+  val quot : z -> z -> z
+  
+  val rem : z -> z -> z
+  
+  val even : z -> bool
+  
+  val odd : z -> bool
+  
+  val div2 : z -> z
+  
+  val quot2 : z -> z
+  
+  val log2 : z -> z
+  
+  val sqrtrem : z -> (z, z) prod
+  
+  val sqrt : z -> z
+  
+  val gcd : z -> z -> z
+  
+  val ggcd : z -> z -> (z, (z, z) prod) prod
+  
+  val testbit : z -> z -> bool
+  
+  val shiftl : z -> z -> z
+  
+  val shiftr : z -> z -> z
+  
+  val coq_lor : z -> z -> z
+  
+  val coq_land : z -> z -> z
+  
+  val ldiff : z -> z -> z
+  
+  val coq_lxor : z -> z -> z
+  
+  val eq_dec : z -> z -> sumbool
+  
+  module Private_BootStrap : 
+   sig 
+    
+   end
+  
+  val leb_spec0 : z -> z -> reflect
+  
+  val ltb_spec0 : z -> z -> reflect
+  
+  module Private_OrderTac : 
+   sig 
+    module Elts : 
+     sig 
+      type t = z
+     end
+    
+    module Tac : 
+     sig 
+      
+     end
+   end
+  
+  val sqrt_up : z -> z
+  
+  val log2_up : z -> z
+  
+  module Private_NZDiv : 
+   sig 
+    
+   end
+  
+  module Private_Div : 
+   sig 
+    module Quot2Div : 
+     sig 
+      val div : z -> z -> z
+      
+      val modulo : z -> z -> z
+     end
+    
+    module NZQuot : 
+     sig 
+      
+     end
+   end
+  
+  val lcm : z -> z -> z
+  
+  val eqb_spec : z -> z -> reflect
+  
+  val b2z : bool -> z
+  
+  val setbit : z -> z -> z
+  
+  val clearbit : z -> z -> z
+  
+  val lnot : z -> z
+  
+  val ones : z -> z
+  
+  module Private_Tac : 
+   sig 
+    
+   end
+  
+  module Private_Rev : 
+   sig 
+    module ORev : 
+     sig 
+      type t = z
+     end
+    
+    module MRev : 
+     sig 
+      val max : z -> z -> z
+     end
+    
+    module MPRev : 
+     sig 
+      module Private_Tac : 
+       sig 
+        
+       end
+     end
+   end
+  
+  module Private_Dec : 
+   sig 
+    val max_case_strong :
+      z -> z -> (z -> z -> __ -> 'a1 -> 'a1) -> (__ -> 'a1) -> (__ -> 'a1) ->
+      'a1
+    
+    val max_case :
+      z -> z -> (z -> z -> __ -> 'a1 -> 'a1) -> 'a1 -> 'a1 -> 'a1
+    
+    val max_dec : z -> z -> sumbool
+    
+    val min_case_strong :
+      z -> z -> (z -> z -> __ -> 'a1 -> 'a1) -> (__ -> 'a1) -> (__ -> 'a1) ->
+      'a1
+    
+    val min_case :
+      z -> z -> (z -> z -> __ -> 'a1 -> 'a1) -> 'a1 -> 'a1 -> 'a1
+    
+    val min_dec : z -> z -> sumbool
+   end
+  
+  val max_case_strong : z -> z -> (__ -> 'a1) -> (__ -> 'a1) -> 'a1
+  
+  val max_case : z -> z -> 'a1 -> 'a1 -> 'a1
+  
+  val max_dec : z -> z -> sumbool
+  
+  val min_case_strong : z -> z -> (__ -> 'a1) -> (__ -> 'a1) -> 'a1
+  
+  val min_case : z -> z -> 'a1 -> 'a1 -> 'a1
+  
+  val min_dec : z -> z -> sumbool
+ end
+
+type 'x compare0 =
 | LT
 | EQ
 | GT
@@ -143,7 +948,7 @@ module type OrderedType =
  sig 
   type t 
   
-  val compare : t -> t -> t compare
+  val compare : t -> t -> t compare0
   
   val eq_dec : t -> t -> sumbool
  end
@@ -172,7 +977,7 @@ module type UsualOrderedType =
  sig 
   type t 
   
-  val compare : t -> t -> t compare
+  val compare : t -> t -> t compare0
   
   val eq_dec : t -> t -> sumbool
  end
@@ -181,7 +986,7 @@ module Z_as_OT :
  sig 
   type t = z
   
-  val compare : z -> z -> z compare
+  val compare : z -> z -> z compare0
   
   val eq_dec : z -> z -> sumbool
  end
@@ -213,7 +1018,7 @@ module type S =
   
   val diff : t -> t -> t
   
-  val compare : t -> t -> t compare
+  val compare : t -> t -> t compare0
   
   val equal : t -> t -> bool
   
@@ -321,7 +1126,7 @@ module Raw :
   
   val choose : t -> elt option
   
-  val compare : t -> t -> t compare
+  val compare : t -> t -> t compare0
  end
 
 module MakeRaw : 
@@ -394,14 +1199,14 @@ module MakeRaw :
     
     val choose : t -> elt option
     
-    val compare : t -> t -> t compare
+    val compare : t -> t -> t compare0
    end
   
   module E : 
    sig 
     type t = X.t
     
-    val compare : t -> t -> t compare
+    val compare : t -> t -> t compare0
     
     val eq_dec : t -> t -> sumbool
    end
@@ -483,7 +1288,7 @@ module MakeRaw :
   
   val partition : (elt -> bool) -> t -> (t, t) prod
   
-  val compare : t -> t -> t compare
+  val compare : t -> t -> t compare0
   
   val eq_dec : t -> t -> sumbool
  end
@@ -495,7 +1300,7 @@ module Make :
    sig 
     type t = X.t
     
-    val compare : t -> t -> t compare
+    val compare : t -> t -> t compare0
     
     val eq_dec : t -> t -> sumbool
    end
@@ -569,14 +1374,14 @@ module Make :
       
       val choose : t -> elt option
       
-      val compare : t -> t -> t compare
+      val compare : t -> t -> t compare0
      end
     
     module E : 
      sig 
       type t = X.t
       
-      val compare : t -> t -> t compare
+      val compare : t -> t -> t compare0
       
       val eq_dec : t -> t -> sumbool
      end
@@ -658,7 +1463,7 @@ module Make :
     
     val partition : (elt -> bool) -> t -> (t, t) prod
     
-    val compare : t -> t -> t compare
+    val compare : t -> t -> t compare0
     
     val eq_dec : t -> t -> sumbool
    end
